kore/src/theories/TrialSubsorts.v
@@ -1,0 +1,143 @@
+From MatchingLogic Require Export stdpp_ext.
+From Kore Require Export Semantics.
+Import Signature.StringVariables.
+Import Kore.Syntax.Notations.
+
+From Coq Require Import ZArith.
+
+Open Scope kore_scope.
+Open Scope hlist_scope.
+Open Scope string_scope.
+
+Ltac autorewrite_set :=
+  repeat (
+    rewrite intersection_top_l_L +
+    rewrite intersection_top_r_L +
+    rewrite union_empty_l_L +
+    rewrite union_empty_r_L +
+    rewrite propset_difference_neg +
+    rewrite propset_union_simpl +
+    rewrite propset_intersection_simpl +
+    rewrite singleton_subseteq_l
+  ).
+
+Ltac basic_simplify_krule :=
+  simpl;
+  eval_helper;
+  repeat rewrite_app_ext;
+  autorewrite_set.
+Ltac simplify_krule :=
+  basic_simplify_krule;
+  apply propset_top_elem_of_2;
+  intro;
+  apply elem_of_PropSet;
+  repeat rewrite elem_of_PropSet;
+  repeat rewrite singleton_subseteq;
+  repeat rewrite singleton_eq.
+
+
+Ltac abstract_var := 
+  match goal with
+    | [|- context [evar_valuation ?σ ?s]] =>
+      let x := fresh "var" in
+      let Hx := fresh "Hvar" in
+        remember (evar_valuation σ s) as x eqn:Hx (*;
+        clear Hx;
+        revert x *)
+    end.
+
+Module T.
+
+  (* We have two sorts: natural numbers and bools *)
+  Inductive DemoSorts :=
+  | SortNat
+  | SortBool
+  | SortK
+  | SortKItem
+  | SortList.
+
+  (* We prove decidable equality and finiteness of the type above. *)
+  Instance DemoSorts_eq_dec : EqDecision DemoSorts.
+  Proof. solve_decision. Defined.
+  Program Instance DemoSorts_finite : finite.Finite DemoSorts := {
+    enum := [SortNat; SortBool; SortK; SortKItem; SortList];
+  }.
+  Next Obligation. compute_done. Defined.
+  Final Obligation. destruct x; set_solver. Defined.
+
+
+  Inductive DemoSyms :=
+  | SymZero
+  | SymSucc
+  | SymAdd
+  | SymTrue
+  | SymFalse
+  | SymIsList
+  | SymNil
+  | SymCons
+  | SymInList.
+
+  (* We prove decidable equality and finiteness of the type above. *)
+  Instance DemoSyms_eq_dec : EqDecision DemoSyms.
+  Proof. solve_decision. Defined.
+  Program Instance DemoSyms_finite : finite.Finite DemoSyms := {
+    enum := [SymZero;SymSucc;SymAdd;SymTrue;
+    SymFalse;SymIsList;SymNil;SymCons;SymInList];
+  }.
+  Next Obligation. compute_done. Defined.
+  Final Obligation. destruct x; set_solver. Defined.
+
+  (* In the signature, we need to define the sorts, the variable types,
+     and the typing/sorting rules for symbols: *)
+  Program Instance DemoSignature : Signature := {|
+    sorts := {|
+      sort := DemoSorts;
+    |};
+    variables := StringVariables;
+    symbols := {|
+      symbol := DemoSyms;
+      arg_sorts :=
+        fun σ => match σ with
+                 | SymZero => []
+                 | SymSucc => [SortNat]
+                 | SymAdd => [SortNat; SortNat]
+                 | SymTrue => []
+                 | SymFalse => []
+                 | SymIsList => [SortK]
+                 | SymNil => []
+                 | SymCons => [SortKItem; SortList]
+                 | SymInList => [SortKItem; SortList]
+                 end;
+      ret_sort := fun σ => match σ with
+                           | SymZero | SymSucc | SymAdd => SortNat
+                           | SymTrue | SymFalse => SortBool
+                           | SymNil | SymCons => SortList
+                           | SymInList | SymIsList => SortBool
+                           end;
+    |};
+  |}.
+
+  (* Definition carrier s :=
+    match s with
+    | SortNat => nat
+    | SortBool => bool
+    | SortList => ?
+    | SortK => ?
+    | SortKItem => ?
+    end. *)
+  Inductive carrier : DemoSorts -> Set :=
+(*   | c_true : carrier SortBool
+  | c_false : carrier SortBool
+  | c_zero : carrier SortNat
+  | c_succ : carrier SortNat -> carrier SortNat *)
+  | c_nat (n : nat) : carrier SortNat
+  | c_bool (b : bool) : carrier SortBool
+  | c_nil : carrier SortList
+  | c_cons {A} : carrier A -> carrier SortList -> carrier SortList.
+
+  Check c_nat 1.
+  Check c_nil.
+  Check c_cons (c_nat 1) c_nil.
+  Check c_cons (c_nat 1) (c_cons (c_bool false) c_nil).
+  Check c_cons (c_nat 1) (c_cons (c_bool false) (c_cons (c_cons (c_nat 1) c_nil) c_nil)).
+
